finish subst proof

lambda/coq/lambda.v
@@ -1,4 +1,5 @@
 Require Import Arith.
+Require Import Lia.
 
 Inductive lambda : Type :=
   | Var : nat -> lambda
@@ -8,15 +9,12 @@ Inductive lambda : Type :=
 
 (* Lifting *)
 
-Definition relocate (i k n : nat) :=
-  if k <=? i
-  then n + i
-  else i.
-
-
 Fixpoint lift_rec (L : lambda) (k n: nat) : lambda :=
   match L with
-  | Var i => Var (relocate i k n)
+  | Var i =>
+      if k <=? i
+      then Var (n + i)
+      else Var i
   | Abs M => Abs (lift_rec M (S k) n)
   | App M N => App (lift_rec M k n) (lift_rec N k n)
   end.
@@ -25,20 +23,18 @@ Definition lift (n : nat) (N : lambda) := lift_rec N 0 n.
 
 (* Substitution *)
 
-Definition insert_Ref (N : lambda) (i k : nat) :=
-       if k <? i then Var (pred i)
-  else if k =? i then lift k N
-                 else Var i.
-
-Fixpoint subst_rec (L N : lambda) (k : nat): lambda :=
+Fixpoint subst_rec (p: nat) (L N : lambda) (k : nat)  : lambda :=
   match L with
-  | Var i => insert_Ref N i k
-  | Abs M => Abs (subst_rec M N (S k))
-  | App M M' => App (subst_rec M N k) (subst_rec M' N k)
+  | Var i =>
+    if k + p =? i then lift p N
+                  else Var i
+  | Abs M    => Abs (subst_rec (S p) M N k)
+  | App M M' => App (subst_rec p M N k) (subst_rec p M' N k)
   end.
 
-Definition subst (N M : lambda) := subst_rec M N 0.
+Definition subst := subst_rec 0.
 
+Notation "t '[' x '<-' u ']'" := (subst t u x) (at level 20).
 
 (* star reduction *)
 
@@ -50,11 +46,157 @@ Inductive star (R : lambda -> lambda -> Prop) : lambda -> lambda -> Prop :=
 (* Beta-reduction *)
 
 Inductive b_red : lambda -> lambda -> Prop :=
-  | beta    : forall M N, b_red (App (Abs M) N) (subst M N)
+  | beta    : forall M N, b_red (App (Abs M) N) (subst M N 0)
   | b_abs   : forall M M', b_red M M' -> b_red (Abs M) (Abs M')
   | b_app1  : forall M M' N, b_red M M' -> b_red (App M N) (App M' N)
   | b_app2  : forall M N N', b_red N N' -> b_red (App M N) (App M N')
 .
 
 Definition b_star := star b_red.
+
+(* free *)
+Fixpoint free_rec n' (L : lambda) n :=
+  match L with
+  | Var v => n + n' =? v
+  | Abs l => free_rec (S n') l n
+  | App l1 l2 => if free_rec n' l1 n then true else free_rec n' l2 n
+  end.
+
+Definition free := free_rec 0.
+
+Lemma lift_neutral:
+  forall L n, lift_rec L n 0 = L.
+Proof.
+  induction L; intros n'; unfold lift; simpl; auto.
+  - case (n' <=? n); auto.
+  - f_equal. apply IHL.
+  - f_equal; [apply IHL1 | apply IHL2].
+Qed.
+
+Lemma subst_free_rec:
+  forall L V x n,
+  free_rec n L x = false ->
+  subst_rec n L V x = L.
+Proof.
+  induction L; intros V x n' Free.
+  - simpl in *. now rewrite Free.
+  - simpl in *. f_equal. now apply IHL.
+  - simpl in *.
+    case (free_rec n' L1 x) eqn:Free1. discriminate Free.
+    f_equal; [apply IHL1 | apply IHL2]; auto.
+Qed.
+
+Lemma free_lift_add:
+  forall V x y z,
+  free_rec x V y = false ->
+  free_rec (x + z) (lift_rec V x z) y = false.
+Proof.
+  induction V; intros x y z Free; simpl.
+  - simpl in Free.
+    case (x <=? n) eqn:Hxn.
+    + simpl. rewrite Nat.eqb_neq in *. lia.
+    + simpl. rewrite Nat.eqb_neq, Nat.leb_gt in *. lia.
+  - simpl in Free. rewrite <- Nat.add_succ_l. now apply IHV.
+  - simpl in Free.
+    case (free_rec x V1 y) eqn:Free2. discriminate.
+    rewrite IHV1; auto.
+Qed.
+
+Lemma free_lift:
+  forall V x z,
+  free V x = false ->
+  free_rec z (lift_rec V 0 z) x = false.
+Proof.
+  induction V; intros x z Hf.
+  - unfold free in Hf. simpl in *.
+    rewrite Nat.eqb_neq in *. lia.
+  - unfold free in *. simpl in *.
+    rewrite <- Nat.add_1_r, Nat.add_comm.
+    now apply free_lift_add.
+  - unfold free in Hf. simpl in *.
+    case (free_rec 0 V1 x) eqn:Hf1. discriminate.
+    rewrite IHV1; auto.
+Qed.
+
+Lemma lift_lift:
+  forall V n0 z n,
+  lift_rec V n (n0 + z) = lift_rec (lift_rec V n n0) (n + n0) z.
+Proof.
+  induction V; intros n0 z n'.
+  - simpl. case (n' <=? n) eqn:Hlt.
+    + simpl. assert (H: n' + n0 <=? n0 + n = true).
+      { rewrite Nat.leb_le in *. lia. }
+      rewrite H. f_equal. lia.
+    + simpl. assert (H: n' + n0 <=? n = false).
+      { rewrite Nat.leb_gt in *. lia. }
+      now rewrite H.
+  - simpl. f_equal. apply IHV.
+  - simpl. f_equal; [apply IHV1 | apply IHV2]. 
+Qed.
+
+Lemma sub_lift:
+  forall U V z y n,
+  subst_rec (z + n) (lift_rec U n z) V y = lift_rec (subst_rec n U V y) n z.
+Proof.
+  induction U; intros *.
+  - simpl.
+    case (n0 <=? n) eqn:Hle.
+    + simpl. rewrite (Nat.add_comm z n0), Nat.add_assoc, Nat.add_comm.
+      case (y + n0 =? n) eqn:Heq.
+      * assert (Heqz: z + (y + n0) =? z + n = true).
+        { rewrite Nat.eqb_eq in *. lia. }
+        rewrite Heqz. unfold lift.
+        apply lift_lift.
+      * assert (Heqz: z + (y + n0) =? z + n = false).
+        { rewrite Nat.eqb_neq in *. lia. }
+        rewrite Heqz. simpl. now rewrite Hle.
+    + assert (Hneq: y + n0 =? n = false).
+      { rewrite Nat.eqb_neq. rewrite Nat.leb_gt in Hle. lia. }
+      rewrite Hneq. simpl. rewrite Hle.
+      assert (Hneq': y + (z + n0) =? n = false).
+      { rewrite Nat.eqb_neq. rewrite Nat.leb_gt in Hle. lia. }
+      now rewrite Hneq'.
+  - simpl. f_equal. rewrite <- Nat.add_succ_r. apply IHU.
+  - simpl. f_equal; [apply IHU1 | apply IHU2].
+Qed.
+
+Lemma comm_subst_rec:
+  forall T U V x y n,
+  y <> x ->
+  free V x = false ->
+  subst_rec n (subst_rec n T U x) V y =
+  subst_rec n (subst_rec n T V y) (subst_rec 0 U V y) x.
+Proof.
+  induction T; intros U V x y z Neq_x_y X_free_V; unfold subst; simpl.
+  - case (x + z =? n) eqn:Hxn.
+    + rewrite Nat.eqb_eq in Hxn. subst.
+      rewrite <- Nat.eqb_neq in Neq_x_y.
+      simpl.
+      assert (Hyzx: y + z =? x + z = false) by (rewrite Nat.eqb_neq in *; lia).
+      rewrite Hyzx. simpl.
+      rewrite Nat.eqb_refl.
+      unfold lift.
+      rewrite <- (Nat.add_0_r z) at 1.
+      apply sub_lift.
+    + case (y + z =? n) eqn:Hyn.
+      * rewrite Nat.eqb_eq in Hyn; subst.
+        simpl. rewrite Nat.eqb_refl.
+        unfold lift. rewrite subst_free_rec; auto.
+        now apply free_lift.
+      * simpl. now rewrite Hxn, Hyn.
+  - f_equal. now apply IHT.
+  - f_equal; [apply IHT1 | apply IHT2]; auto.
+Qed.
+
+Theorem comm_subst:
+  forall T U V x y,
+  y <> x ->
+  free V x = false ->
+  T[x <- U][y <- V] =
+  T[y <- V][x <- U[y <- V]].
+Proof.
+  intros * H F.
+  unfold subst.
+  now apply comm_subst_rec.
+Qed.
 
